lib_list/Selectors.LList.fsti
@@ -16,8 +16,11 @@ let t (a:Type0) = ref (cell a)
 
 (* Helpers to manipulate cells while keeping its definition abstract *)
 
+inline_for_extraction noextract
 val get_next (#a:Type0) (c:cell a) : t a
+inline_for_extraction noextract
 val get_data (#a:Type0) (c:cell a) : a
+inline_for_extraction noextract
 val mk_cell (#a:Type0) (n: t a) (d:a)
   : Pure (cell a)
     (requires True)
@@ -26,9 +29,11 @@ val mk_cell (#a:Type0) (n: t a) (d:a)
       get_data c == d)
 
 /// The null list pointer
+inline_for_extraction noextract
 val null_t (#a:Type) : t a
 
 /// Lifting the null pointer check to empty lists
+inline_for_extraction noextract
 val is_null_t (#a:Type) (ptr:t a) : (b:bool{b <==> ptr == null_t})
 
 /// Separation logic predicate stating that reference [r] points to a valid list in memory
@@ -51,41 +56,42 @@ let llist (#a:Type0) (p : a -> vprop) (r:t a) = VUnit (llist' p r)
 /// calling a variant of the framing tactic, as defined in Steel.Effect.Common
 [@@ __steel_reduce__]
 let v_llist (#a:Type0) (#p2:vprop) (p : a -> vprop) (r:t a)
-  //(h:rmem p{FStar.Tactics.with_tactic selector_tactic (can_be_split p (llist r) /\ True)}) : GTot (list a)
   (h:rmem p2{FStar.Tactics.with_tactic selector_tactic (can_be_split p2 (llist p r) /\ True)}) : GTot (list a)
   = h (llist p r)
 
 (** Stateful lemmas to fold and unfold the llist predicate **)
 
-val intro_llist_nil (a:Type0) (p : a -> vprop)
-  : Steel unit emp (fun _ -> llist p (null_t #a))
-          (requires fun _ -> True)
-          (ensures fun _ _ h1 -> v_llist #a p null_t h1 == [])
+val intro_llist_nil (#opened:inames) (#a:Type0) (p : a -> vprop)
+  : SteelGhost unit opened
+    emp (fun _ -> llist p (null_t #a))
+    (requires fun _ -> True)
+    (ensures fun _ _ h1 -> v_llist #a p null_t h1 == [])
 
-val elim_llist_nil (#a:Type0) (p : a -> vprop) (ptr:t a)
-  : Steel unit (llist p ptr) (fun _ -> llist p ptr)
-          (requires fun _ -> ptr == null_t)
-          (ensures fun h0 _ h1 ->
-            v_llist p ptr h0 == v_llist p ptr h1 /\
-            v_llist p ptr h1 == [])
+val elim_llist_nil (#opened:inames) (#a:Type0) (p : a -> vprop) (ptr:t a)
+  : SteelGhost unit opened
+  (llist p ptr) (fun _ -> llist p ptr)
+  (requires fun _ -> ptr == null_t)
+  (ensures fun h0 _ h1 ->
+    v_llist p ptr h0 == v_llist p ptr h1 /\
+    v_llist p ptr h1 == [])
 
-val cons_is_not_null (#a:Type0) (p : a -> vprop) (ptr:t a)
-  : Steel unit (llist p ptr) (fun _ -> llist p ptr)
-             (requires fun h -> Cons? (v_llist p ptr h))
-             (ensures fun h0 _ h1 ->
-               v_llist p ptr h0 == v_llist p ptr h1 /\
-               ptr =!= null_t)
+val cons_is_not_null (#opened:inames) (#a:Type0) (p : a -> vprop) (ptr:t a)
+  : SteelGhost unit opened
+  (llist p ptr) (fun _ -> llist p ptr)
+  (requires fun h -> Cons? (v_llist p ptr h))
+  (ensures fun h0 _ h1 ->
+    v_llist p ptr h0 == v_llist p ptr h1 /\
+    ptr =!= null_t)
 
-//val intro_llist_cons (#a:Type0) (p : a -> vprop) (ptr1 ptr2:t a)
-//  : Steel unit (vptr ptr1 `star` llist p ptr2)
-//                  (fun _ -> llist p ptr1)
-//                  (requires fun h -> get_next (sel ptr1 h) == ptr2)
-//                  (ensures fun h0 _ h1 -> v_llist p ptr1 h1 == (get_data (sel ptr1 h0)) :: v_llist p ptr2 h0)
+// val null_is_nil
+// val nil_is_null
+// val not_null_is_cons
 
-val intro_llist_cons (#a:Type0) (p : a -> vprop)
-  (ptr1 ptr2:t a) (x: a)
-  //(y: t_of (p (get_data x)))
-  : Steel unit
+val pack_list (#opened:inames) (#a:Type0)
+  (p: a -> vprop)
+  (ptr1 ptr2: t a)
+  (x: a)
+  : SteelGhost unit opened
   (vptr ptr1 `star`
   llist p ptr2 `star`
   p x)
@@ -93,25 +99,23 @@ val intro_llist_cons (#a:Type0) (p : a -> vprop)
   (requires fun h ->
     get_next (sel ptr1 h) == ptr2 /\
     x == get_data (sel ptr1 h)
-    ///\
-    //y == sel (sel_of (p (get_data x))) h
   )
   (ensures fun h0 _ h1 ->
-  v_llist p ptr1 h1 == (get_data (sel ptr1 h0)) :: v_llist p ptr2 h0)
+    v_llist p ptr1 h1 ==
+      (get_data (sel ptr1 h0)) :: v_llist p ptr2 h0)
 
-
-
-val tail (#a:Type0) (p : a -> vprop) (ptr:t a)
-  : Steel (cell a) (llist p ptr)
-                   (fun n -> vptr ptr `star` llist p (get_next n) `star` p (get_data n))
-                   (requires fun _ -> ptr =!= null_t)
-                   (ensures fun h0 n h1 ->
-                     Cons? (v_llist p ptr h0) /\
-                     v_llist p ptr h0 ==
-                       (get_data (sel ptr h1)) :: (v_llist p (get_next n) h1) /\
-                      sel ptr h1 == n)
-                     //sel ptr h1 == mk_cell n (L.hd (v_llist p ptr h0)) /\
-                     //v_llist p n h1 == L.tl (v_llist p ptr h0))
+val unpack_list (#a:Type0)
+  (p: a -> vprop)
+  (ptr:t a)
+  : Steel (cell a)
+  (llist p ptr)
+  (fun n -> vptr ptr `star` llist p (get_next n) `star` p (get_data n))
+  (requires fun _ -> ptr =!= null_t)
+  (ensures fun h0 n h1 ->
+    Cons? (v_llist p ptr h0) /\
+    v_llist p ptr h0 ==
+      (get_data (sel ptr h1)) :: (v_llist p (get_next n) h1) /\
+     sel ptr h1 == n)
 
 (*)
 (** A variant of lists with an additional indirection pointer to enable in-place operations **)
